Papers/Tree/SlideSnippets.thy
@@ -6,7 +6,7 @@ notation (latex)
   kind ("_\<llangle>_\<rrangle>")
 
 notation (latex)
-  TreeToGraph.ord_IRExpr_inst.less_eq_IRExpr ("_ \<longmapsto> _")
+  IRTreeEval.ord_IRExpr_inst.less_eq_IRExpr ("_ \<longmapsto> _")
 
 text_raw \<open>\Snip{abstract-syntax-tree}%
 @{datatype[display,margin=45] IRExpr}
